examples/kv_parsing/Serializer.fst
@@ -17,6 +17,7 @@ open PureEncoder
 (* NOTE: I'm using ser out of laziness, but they should NOT be abbreviated, we
 can serialize everywhere *)
 
+unfold
 let offset_into (buf:bslice) = off:U32.t{U32.v off <= U32.v buf.len}
 
 let serialized (enc:bytes) (buf:bslice) (r:option (offset_into buf)) (h0 h1:mem) :
@@ -40,6 +41,7 @@ let buffer_fun (inputs:erased (TSet.set bslice)) =
 let disjoint_in (h:mem) (inputs:TSet.set bslice) (buf:bslice) =
   forall b. TSet.mem b inputs ==> live h b /\ B.disjoint b.p buf.p
 
+unfold
 let serializer_any (inputs:erased (TSet.set bslice))
                    (enc: buffer_fun inputs) =
   buf:bslice ->
@@ -55,6 +57,7 @@ let serializer_any (inputs:erased (TSet.set bslice))
            as_seq h0 b == as_seq h1 b) /\
         serialized (enc h1) buf r h0 h1))
 
+unfold
 let serializer (enc:erased bytes) = serializer_any (hide TSet.empty) (fun _ -> reveal enc)
 
 let serializer_1 (input:bslice) (enc: buffer_fun (hide (TSet.singleton input))) =
